lawyer/nonblocking/wait_free_spec_defs.v
@@ -1,0 +1,30 @@
+From iris.proofmode Require Import tactics.
+(* From lawyer.examples Require Import orders_lib. *)
+(* From lawyer.nonblocking.logrel Require Import logrel. *)
+From trillium.program_logic Require Import weakestpre. 
+From heap_lang Require Import heap_lang_defs lang notation.
+From lawyer.obligations Require Import obligations_resources env_helpers obligations_model.
+
+
+
+Definition wait_free_method
+  {M} {EM: ExecutionModel heap_lang M} {Σ} `{OP: OP_HL DegO LvlO LIM}
+  {OHE: OM_HL_Env OP EM Σ}
+  (m: val) (d: DegO) (F: nat)
+  : iProp Σ :=
+  ∀ τ π q (a: val), 
+    {{{ cp_mul π d F ∗ th_phase_frag τ π q }}}
+      App m a @ τ
+    {{{ v, RET v; th_phase_frag τ π q }}}. 
+
+(* TODO: unify *)
+Definition wait_free_method_gen
+  {M} {EM: ExecutionModel heap_lang M} {Σ} `{OP: OP_HL DegO LvlO LIM}
+  {OHE: OM_HL_Env OP EM Σ}
+  (m: val) (d: DegO) (F: nat) (P Q: val -> Prop)
+  : iProp Σ :=
+  ∀ τ π q (a: val), 
+    {{{ cp_mul π d F ∗ th_phase_frag τ π q ∗ ⌜ P a ⌝ }}}
+      App m a @ τ
+    {{{ v, RET v; th_phase_frag τ π q ∗ ⌜ Q v ⌝ }}}. 
+  
